CompileModule compiles

platform/Depl/CompileModule.v
@@ -4,7 +4,7 @@ Require Import Bool.
 
 Require Import AutoSep Wrap Malloc.
 
-Require Import Depl.Logic Depl.Statements Depl.Compile.
+Require Import Depl.Logic Depl.AlgebraicDatatypes Depl.Statements Depl.Compile.
 
 
 (** * Functions *)
@@ -36,518 +36,665 @@ Fixpoint formals (V : vals) (xs : list pr_var) (fE : fo_env) : fo_env :=
     | x :: xs => fo_set (formals V xs fE) (x ++ "0")%string (Dyn (sel V x))
   end.
 
-(** Generic top-level function spec (see [Compile.precond] for comments) *)
-Definition precond (frmls lcls : list pr_var) (pre post : pred) (inBody : bool) : assert :=
-  (Al fE,
-    PRE[V] mallocHeap 0 * predD pre (formals V frmls fE)
-    POST[R] mallocHeap 0 * predD post (fo_set (formals V frmls fE) "result" (Dyn R)))
-  inBody (fun w => w) (if inBody then frmls ++ lcls else frmls) (if inBody then 0 else length lcls).
+Section dts.
+  Variable dts : list datatype.
 
-(** A default function, for when things go horribly wrong *)
-Definition function0 name : Programming.function := {|
-  FName := name;
-  FVars := nil;
-  FReserved := 0;
-  FPrecondition := (st ~> [| False |]);
-  FBody := Skip
-|}.
+  (** Generic top-level function spec (see [Compile.precond] for comments) *)
+  Definition precond (frmls lcls : list pr_var) (pre post : pred) (inBody : bool) : assert :=
+    (Al fE,
+      PRE[V] mallocHeap 0 * predD dts pre (formals V frmls fE)
+      POST[R] mallocHeap 0 * predD dts post (fo_set (formals V frmls fE) "result" (Dyn R)))
+    inBody (fun w => w) (if inBody then frmls ++ lcls else frmls) (if inBody then 7 else 7 + length lcls).
 
-(** Initial symbolic variable assignment *)
-Definition vars0 (xs : list pr_var) : vars := 
-  fun x => if in_dec string_dec x xs then Some (Logic.Var (x ++ "0")%string) else None.
+  (** A default function, for when things go horribly wrong *)
+  Definition function0 name : Programming.function := {|
+    FName := name;
+    FVars := nil;
+    FReserved := 0;
+    FPrecondition := (st ~> [| False |]);
+    FBody := Skip
+  |}.
 
-(** Generating one Bedrock function *)
-Definition compileFunction (f : function) : Programming.function :=
-  let xs := Formals f ++ Locals f in
-  match boundVars (Precondition f), boundVars (Postcondition f) with
-    | Some bvs, Some bvs' => {|
-      FName := Name f;
-      FVars := Formals f;
-      FReserved := length (Locals f);
-      FPrecondition := precond (Formals f) (Locals f) (Precondition f) (Postcondition f) false;
-      FBody := ($[Sp+0] <- Rp;;
-        (fun _ _ =>
-          Structured nil (fun im mn _ => Structured.Assert_ im mn
-            (precond (Formals f) (Locals f) (Precondition f) (Postcondition f) true)));;
-        (fun _ _ => Stmt (map (fun s => s ++ "0")%string xs ++ SpecVars f)
-          bvs bvs' xs (vars0 (Formals f))
-          (Precondition f) (Postcondition f) (Body f) xs 0))%SP
-    |}
-    | _, _ => function0 (Name f)
-  end.
+  (** Initial symbolic variable assignment *)
+  Definition vars0 (xs : list pr_var) : vars := 
+    fun x => if in_dec string_dec x xs then Some (Logic.Var (x ++ "0")%string) else None.
 
-(** Deciding whether a list is duplicate-free *)
-Section NoDup_dec.
-  Variable A : Type.
-  Variable dec : forall x y : A, {x = y} + {x <> y}.
+  (** Generating one Bedrock function *)
+  Definition compileFunction (f : function) : Programming.function :=
+    let xs := Formals f ++ Locals f in
+    match boundVars (Precondition f), boundVars (Postcondition f) with
+      | Some bvs, Some bvs' => {|
+        FName := Name f;
+        FVars := Formals f;
+        FReserved := 7 + length (Locals f);
+        FPrecondition := precond (Formals f) ("_" :: Locals f)
+                                 (Precondition f) (Postcondition f) false;
+        FBody := ($[Sp+0] <- Rp;;
+          (fun _ _ =>
+            Structured nil (fun im mn _ => Structured.Assert_ im mn
+              (precond (Formals f) ("_" :: Locals f) (Precondition f) (Postcondition f) true)));;
+          (fun _ _ => Stmt dts (map (fun s => s ++ "0")%string xs ++ SpecVars f)
+            bvs bvs' xs (vars0 (Formals f))
+            (Precondition f) (Postcondition f) (Body f)
+            (Formals f ++ "_" :: Locals f) 7))%SP
+      |}
+      | _, _ => function0 (Name f)
+    end.
 
-  Hint Constructors NoDup.
+  (** Deciding whether a list is duplicate-free *)
+  Section NoDup_dec.
+    Variable A : Type.
+    Variable dec : forall x y : A, {x = y} + {x <> y}.
 
-  Definition NoDup_dec : forall ls : list A, {NoDup ls} + {~NoDup ls}.
-  Proof.
-    refine (fix NoDup_dec (ls : list A) : {NoDup ls} + {~NoDup ls} :=
-      match ls return {NoDup ls} + {~NoDup ls} with
-        | nil => left _
-        | x :: ls' => if in_dec dec x ls' then right _ else
-          if NoDup_dec ls' then left _ else right _
-      end); clear NoDup_dec; abstract (eauto; inversion_clear 1; tauto).
-  Defined.
-End NoDup_dec.
+    Hint Constructors NoDup.
 
-(** Does a list of variables include any ending in "0"?
-  * We're using that convention for our automatically generated variables,
-  * so it's a no-no for the programmer to use it. *)
+    Definition NoDup_dec : forall ls : list A, {NoDup ls} + {~NoDup ls}.
+    Proof.
+      refine (fix NoDup_dec (ls : list A) : {NoDup ls} + {~NoDup ls} :=
+        match ls return {NoDup ls} + {~NoDup ls} with
+          | nil => left _
+          | x :: ls' => if in_dec dec x ls' then right _ else
+            if NoDup_dec ls' then left _ else right _
+        end); clear NoDup_dec; abstract (eauto; inversion_clear 1; tauto).
+    Defined.
+  End NoDup_dec.
 
-Fixpoint anyZero (x : fo_var) : bool :=
-  match x with
-    | "" => false
-    | "0" => true
-    | String _ x' => anyZero x'
-  end.
+  (** Does a list of variables include any ending in "0"?
+    * We're using that convention for our automatically generated variables,
+    * so it's a no-no for the programmer to use it. *)
 
-Fixpoint anyZeros (xs : list fo_var) : bool :=
-  match xs with
-    | nil => false
-    | x :: xs' => anyZero x || anyZeros xs'
-  end.
+  Fixpoint anyZero (x : fo_var) : bool :=
+    match x with
+      | "" => false
+      | "0" => true
+      | String _ x' => anyZero x'
+    end.
 
-(** A computable syntactic well-formedness check... *)
-Definition functionWf (f : function) : bool :=
-  let xs := Formals f ++ Locals f in
-  let fvs := map (fun s => s ++ "0")%string xs ++ SpecVars f in
-  if in_dec string_dec "rp" xs
-    then false
-  else if in_dec string_dec "result" fvs
-    then false
-  else if (if NoDup_dec _ string_dec xs then false else true)
-    then false
-  else if anyZeros (SpecVars f)
-    then false
-  else match boundVars (Precondition f), boundVars (Postcondition f) with
+  Fixpoint anyZeros (xs : list fo_var) : bool :=
+    match xs with
+      | nil => false
+      | x :: xs' => anyZero x || anyZeros xs'
+    end.
+
+  Fixpoint good_vars (xs : list fo_var) : bool :=
+    match xs with
+      | nil => true
+      | x :: xs => match x with
+                     | String "_" _ => false
+                     | _ => good_vars xs
+                   end
+    end.
+
+  (** A computable syntactic well-formedness check... *)
+  Definition functionWf (f : function) : bool :=
+    let xs' := Formals f ++ Locals f in
+    let xs := Formals f ++ "_" :: Locals f in
+    let fvs := map (fun s => s ++ "0")%string xs' ++ SpecVars f in
+    notInList "rp" xs' && notInList "result" fvs
+    && (if NoDup_dec _ string_dec xs' then true else false)
+    && negb (anyZeros (SpecVars f)) && notInList "result" (SpecVars f)
+    && match boundVars (Precondition f), boundVars (Postcondition f) with
          | Some bvs, Some bvs' =>
-           if in_dec string_dec "result" bvs
-             then false
-           else if in_dec string_dec "result" bvs'
-             then false
-           else notsInList bvs fvs && notsInList bvs' ("result" :: fvs)
+           notInList "result" bvs && notInList "result" bvs'
+           && notInList "this" bvs && notInList "this" bvs'
+           && notsInList bvs fvs && notsInList bvs' ("result" :: fvs)
+           && good_vars bvs && good_vars bvs'
+           && good_vars (Formals f) && good_vars (Locals f)
+           && notInList "this" (SpecVars f)
          | _, _ => false
        end.
 
-(** ...and a residual part, for what we ask the user to prove *)
-Definition functionVc (f : function) : list Prop :=
-  let xs := Formals f ++ Locals f in
-  let fvs := map (fun s => s ++ "0")%string xs ++ SpecVars f in
-    stmtV xs (Body f)
-    :: wellScoped fvs (Precondition f)
-    :: wellScoped ("result" :: fvs) (Postcondition f)
-    :: stmtD (normalize (Precondition f))
-    (normalize (Postcondition f)) fvs xs (vars0 (Formals f)) (Body f) (fun _ => False)
-    :: nil.
+  Variable dts' : list ndatatype.
 
-(** Combined syntactic check for all functions *)
-Fixpoint functionsWf (fs : list function) : bool :=
-  match fs with
-    | nil => true
-    | f :: fs' => functionWf f && functionsWf fs'
-  end.
+  (** ...and a residual part, for what we ask the user to prove *)
+  Definition functionVc (f : function) : list Prop :=
+    let xs := Formals f ++ Locals f in
+    let fvs := map (fun s => s ++ "0")%string xs ++ SpecVars f in
+      stmtV dts' xs (Body f)
+      :: wellScoped fvs (Precondition f)
+      :: wellScoped ("result" :: fvs) (Postcondition f)
+      :: stmtD dts' xs (vars0 (Formals f)) fvs (normalize (Precondition f))
+      (normalize (Postcondition f)) "_D" (Body f) (fun _ _ _ _ _ => False)
+      :: nil.
 
-(** Combine the VCs of all functions. *)
-Fixpoint makeVcs (fs : list function) : list Prop :=
-  match fs with
-    | nil => nil
-    | f :: fs' => functionVc f ++ makeVcs fs'
-  end.
+  (** Combined syntactic check for all functions *)
+  Fixpoint functionsWf (fs : list function) : bool :=
+    match fs with
+      | nil => true
+      | f :: fs' => functionWf f && functionsWf fs'
+    end.
 
-Ltac clear_fancier := clear_fancy;
-  repeat match goal with
-           | [ H : context[map] |- _ ] => clear H
-         end.
+  (** Combine the VCs of all functions. *)
+  Fixpoint makeVcs (fs : list function) : list Prop :=
+    match fs with
+      | nil => nil
+      | f :: fs' => functionVc f ++ makeVcs fs'
+    end.
 
-Lemma sel_eta : forall V, sel V = V.
-Proof.
-  auto.
-Qed.
-
-Theorem normalize_sound_fwd : forall p fvs bvs fE,
-  wellScoped fvs p
-  -> boundVars p = Some bvs
-  -> (forall x, In x fvs -> ~In x bvs)
-  -> predD p fE ===> normalD (normalize p) fE.
-Proof.
-  intros.
-  change (predD p fE) with (SubstsH (SNil _ _) (predD p fE)).
-  change (normalD (normalize p) fE) with (SubstsH (SNil _ _) (normalD (normalize p) fE)).
-  eapply normalize_sound_fwd; eauto.
-Qed.
-
-Theorem normalize_sound_bwd : forall p fvs bvs fE,
-  wellScoped fvs p
-  -> boundVars p = Some bvs
-  -> (forall x, In x fvs -> ~In x bvs)
-  -> normalD (normalize p) fE ===> predD p fE.
-Proof.
-  intros.
-  change (predD p fE) with (SubstsH (SNil _ _) (predD p fE)).
-  change (normalD (normalize p) fE) with (SubstsH (SNil _ _) (normalD (normalize p) fE)).
-  eapply normalize_sound_bwd; eauto.
-Qed.
-
-Lemma weaken_predD : forall p xs fE fE',
-  wellScoped xs p
-  -> (forall x, In x xs -> fE x = fE' x)
-  -> predD p fE ===> predD p fE'.
-Proof.
-  intros.
-  change (predD p fE) with (SubstsH (SNil _ _) (predD p fE)).
-  change (predD p fE') with (SubstsH (SNil _ _) (predD p fE')).
-  eapply weaken_predD; eauto.
-Qed.
-
-(** Relate the above definitions to what [StructuredModule] wants. *)
-Theorem makeVcs_correct : forall mn fs0 fs, functionsWf fs = true
-  -> vcs (makeVcs fs)
-  -> vcs (StructuredModule.makeVcs nil fs0
-    (map (fun p => match p with
-                     | {| FName := f; FVars := ns; FReserved := res;
-                       FPrecondition := pre; FBody := ch |} =>
-                     (f, pre, fun im' H => toCmd ch mn H ns res)
-                   end)
-    (map compileFunction fs))).
-Proof.
-  induction fs; simpl; intuition.
-  apply andb_prop in H; intuition.
-  unfold functionWf in H1.
-  unfold compileFunction at 1.
-
-  repeat match goal with
-           | [ H : context[if anyZeros ?X then _ else _] |- _ ] =>
-             case_eq (anyZeros X); intros;
-               match goal with
-                 | [ H' : _ = _ |- _ ] => rewrite H' in *
-               end; try discriminate
-           | [ H : context[if (if ?E then _ else _) then _ else _] |- _ ] => destruct E; try discriminate
-           | [ H : context[if ?E then _ else _] |- _ ] => destruct E; try discriminate
-           | [ H : context[match ?E with None => _ | _ => _ end] |- _ ] => case_eq E; intros;
-             match goal with
-               | [ H' : _ = _ |- _ ] => rewrite H' in *
-             end; try discriminate
-         end.
-  apply andb_prop in H1; intuition idtac.
-  simpl.
-  wrap0.
-
-  post; clear_fancier.
-  assert (In "rp" ("rp" :: Formals a)) by (simpl; tauto).
-  assert (~In "rp" (Formals a)) by (intro; apply n0; eauto using in_or_app).
-  change (sel x1) with x1 in *.
-  unfold lvalIn, regInL in *; simpl in H1.
-  change (LvMem (Indir Sp (natToW O))) with (LvMem (Indir Sp (variablePosition ("rp" :: Formals a) "rp"))) in *.
-  evaluate auto_ext.
-
-  post.
-  assert (forall x4 x v, In x (map (fun s : string => (s ++ "0")%string) (Formals a ++ Locals a) ++ SpecVars a)
-    -> formals x2 (Formals a) x0 x
-    = formals (upd (merge x2 x4 ("rp" :: Formals a)) "rp" v)
-    (Formals a) x0 x).
-  intros.
-  apply in_app_or in H; intuition idtac.
-  apply in_map_iff in H16; destruct H16; intuition subst.
-
-  Lemma append0_invert : forall x y,
-    (x ++ "0" = y ++ "0")%string
-    -> x = y.
-  Proof.
-    induction x; destruct y; simpl in *; intuition.
-    destruct y; discriminate.
-    destruct x; discriminate.
-    injection H; clear H; intros; subst.
-    f_equal; auto.
-  Qed.
-
-  Lemma formals_switch : forall V V' x xs fE,
-    (In x xs -> sel V x = sel V' x)
-    -> formals V xs fE (x ++ "0")%string = formals V' xs fE (x ++ "0")%string.
-  Proof.
-    induction xs; simpl; intuition.
-    unfold fo_set.
-    destruct (string_dec (x ++ "0")%string (a ++ "0")%string); subst; auto.
-    apply append0_invert in e; subst.
-    f_equal; auto.
-  Qed.
-
-  apply formals_switch.
-  apply in_app_or in H17; intuition idtac.
-  rewrite sel_upd_ne.
-  symmetry; apply sel_merge.
-  simpl; tauto.
-  intro; subst.
-  eauto using in_or_app.
-
-  Lemma NoDup_unapp : forall A (ls2 ls1 : list A),
-    NoDup (ls1 ++ ls2)
-    -> forall x, In x ls1 -> In x ls2 -> False.
-  Proof.
-    induction ls1; inversion 1; simpl; intuition (subst; eauto using in_or_app).
-  Qed.
-
-  exfalso; eauto using NoDup_unapp.
-  
-  Lemma anyZero_duh : forall s, anyZero (s ++ "0")%string = true.
-  Proof.
-    induction s; simpl; intuition.
-    destruct a.
-    rewrite IHs.
+  Ltac clear_fancier := clear_fancy;
     repeat match goal with
-             | [ |- (if ?E then _ else _) = _ ] => destruct E; auto
+             | [ H : context[map] |- _ ] => clear H
            end.
-  Qed.
 
-  Lemma formals_irrel : forall V V' x xs fE,
-    anyZero x = false
-    -> formals V xs fE x = formals V' xs fE x.
+  Lemma sel_eta : forall V, sel V = V.
   Proof.
-    induction xs; simpl; intuition.
-    unfold fo_set.
-    destruct (string_dec x (a ++ "0")%string); subst; auto.
-    rewrite anyZero_duh in H; discriminate.
-  Qed.
-
-  Lemma anyZeros_correct : forall x xs, anyZeros xs = false
-    -> In x xs
-    -> anyZero x = false.
-  Proof.
-    induction xs; simpl; intuition subst.
-
-    apply orb_false_iff in H; intuition.
-    apply orb_false_iff in H; intuition.
-  Qed.
-
-  eauto using formals_irrel, anyZeros_correct.
-
-  generalize dependent (map (fun s : string => (s ++ "0")%string) (Formals a ++ Locals a) ++ SpecVars a); intros.
-  clear_fancier.
-  clear H11.
-  change (locals ("rp" :: Formals a) x2 (length (Locals a)) (Regs x Sp))
-    with (locals_in ("rp" :: Formals a) x2 (length (Locals a)) (Regs x Sp)
-      (Locals a) ("rp" :: Formals a ++ Locals a) 0) in *.
-  assert (ok_in ("rp" :: Formals a) (length (Locals a))
-    (Locals a) ("rp" :: Formals a ++ Locals a) 0).
-  repeat split; unfold pr_var; auto; try omega.
-  simpl; constructor; auto.
-  assert (In "rp" ("rp" :: Formals a ++ Locals a)) by (simpl; tauto).
-  change (sel x2) with x2 in *.
-  unfold lvalIn, regInL in *; simpl in H12.
-  change (LvMem (Indir Sp (natToW O))) with (LvMem (Indir Sp (variablePosition ("rp" :: Formals a ++ Locals a) "rp"))) in *.
-  evaluate auto_ext.
-  fold (@app pr_var) in *.
-  descend.
-  rewrite sel_eta.
-  step auto_ext.
-  etransitivity; [ apply himp_star_comm | ]; apply himp_star_frame; try reflexivity.
-  eapply weaken_predD; eauto.
-  eauto.
-  step auto_ext.
-  descend; step auto_ext.
-  instantiate (1 := x6).
-  change (locals ("rp" :: Formals a) x6 (Datatypes.length (Locals a)) (Regs x Sp))
-    with (locals_out ("rp" :: Formals a) x6 (Datatypes.length (Locals a)) (Regs x Sp)
-      (Locals a) ("rp" :: Formals a ++ Locals a) 0).
-  assert (ok_out ("rp" :: Formals a) (Datatypes.length (Locals a))
-    (Locals a) ("rp" :: Formals a ++ Locals a) 0).
-  repeat split; unfold pr_var; auto; try omega.
-  rewrite sel_eta.
-  descend; step auto_ext.
-  eapply weaken_predD; eauto.
-  simpl; intuition (subst; eauto).
-  unfold fo_set.
-  destruct (string_dec x6 "result"); subst; auto.
-  symmetry; auto.  
-
-
-  post.
-  generalize dependent (map (fun s : string => (s ++ "0")%string) (Formals a ++ Locals a) ++ SpecVars a); intros.
-  clear_fancier.
-  clear H11.
-  descend.
-  repeat rewrite sel_eta in *.
-  step auto_ext.
-  fold (@app pr_var).
-  Focus 2.
-  apply himp_star_frame; try reflexivity.
-  eapply normalize_sound_fwd; eauto using notsInList_true.
-
-  Lemma formals_grab : forall V x xs fE,
-    In x xs
-    -> formals V xs fE (x ++ "0")%string = Dyn (sel V x).
-  Proof.
-    induction xs; simpl; intuition (subst; eauto).
-    unfold fo_set.
-    destruct (string_dec (x ++ "0")%string (x ++ "0")%string); subst; congruence.
-    unfold fo_set.
-    destruct (string_dec (x ++ "0")%string (a ++ "0")%string); subst; auto.
-    apply append0_invert in e; subst.
     auto.
   Qed.
 
-  Lemma vars_ok_formals : forall V xs fE,
-    vars_ok (formals V xs fE) V (vars0 xs).
+  Theorem normalize_sound_fwd : forall p fvs bvs fE,
+    wellScoped fvs p
+    -> boundVars p = Some bvs
+    -> (forall x, In x fvs -> ~In x bvs)
+    -> predD dts p fE ===> normalD dts (normalize p) fE.
   Proof.
-    unfold vars_ok, vars0; induction xs; simpl; intuition.
-
-    destruct (string_dec a x); subst.
-    injection H; clear H; intros; subst; simpl.
-    unfold fo_set.
-    destruct (string_dec (x ++ "0") (x ++ "0")); tauto.
-    destruct (in_dec string_dec x xs); try discriminate.
-    injection H; clear H; intros; subst; simpl.
-    unfold fo_set.
-    destruct (string_dec (x ++ "0") (a ++ "0")).
-    apply append0_invert in e; congruence.
-    auto using formals_grab.
+    intros.
+    change (predD dts p fE) with (SubstsH (SNil _ _) (predD dts p fE)).
+    change (normalD dts (normalize p) fE) with (SubstsH (SNil _ _) (normalD dts (normalize p) fE)).
+    eapply normalize_sound_fwd; eauto.
   Qed.
 
-  apply vars_ok_formals.
-  step auto_ext.
-  step auto_ext.
-  descend; step auto_ext.
-  descend; step auto_ext.
-  rewrite sel_eta.
-  step auto_ext.
-  eapply normalize_sound_bwd; eauto using notsInList_true.
+  Theorem normalize_sound_bwd : forall p fvs bvs fE,
+    wellScoped fvs p
+    -> boundVars p = Some bvs
+    -> (forall x, In x fvs -> ~In x bvs)
+    -> normalD dts (normalize p) fE ===> predD dts p fE.
+  Proof.
+    intros.
+    change (predD dts p fE) with (SubstsH (SNil _ _) (predD dts p fE)).
+    change (normalD dts (normalize p) fE) with (SubstsH (SNil _ _) (normalD dts (normalize p) fE)).
+    eapply normalize_sound_bwd; eauto.
+  Qed.
 
+  Lemma weaken_predD : forall p xs fE fE',
+    wellScoped xs p
+    -> (forall x, In x xs -> fE x = fE' x)
+    -> predD dts p fE ===> predD dts p fE'.
+  Proof.
+    intros.
+    change (predD dts p fE) with (SubstsH (SNil _ _) (predD dts p fE)).
+    change (predD dts p fE') with (SubstsH (SNil _ _) (predD dts p fE')).
+    eapply weaken_predD; eauto.
+  Qed.
 
-  hnf; auto.
+  Hypothesis Hnodup : nodup dts.
+  Hypothesis Hndts : ndts_good dts dts'.
+  Hypothesis Hdts : datatypesWf dts.
 
-  unfold vars0 in *.
-  destruct (in_dec string_dec x (Formals a)); auto; try congruence.
-  injection H; clear H; intros; subst; simpl.
-  apply H1.
-  apply in_or_app; left.
-  apply in_map_iff; eauto using in_or_app.
-
-  eauto using notsInList_true.
-
-  subst; tauto.
-
-  apply in_app_or in H12; intuition idtac.
-  apply in_map_iff in H1; destruct H1; intuition subst.
-  apply in_app_or in H14; intuition idtac.
-  eapply notsInList_true in H7.
-  tauto.
-  apply H.
-  right.
-  apply in_or_app; left.
-  apply in_map_iff.
-  eauto using in_or_app.
-  eapply notsInList_true in H7.
-  tauto.
-  apply H.
-  right.
-  apply in_or_app; left.
-  apply in_map_iff.
-  eauto using in_or_app.
-  eapply notsInList_true in H7.
-  tauto.
-  apply H.
-  right.
-  apply in_or_app; auto.
-Qed.
-
-
-(** * Modules *)
-
-(** A named group of functions *)
-Record module := {
-  MName : string;
-  Functions : list function
-}.
-
-(** Generating a full module *)
-Section compileModule.
-  Variable m : module.
-
-  Definition compileModule : XCAP.module :=
-    bmodule_ nil (MName m) (map compileFunction (Functions m)).
-
-  Lemma preserve_None : forall fs,
-    fold_left
-    (fun (mOpt : option (LabelMap.t unit)) (f : function) =>
-      match mOpt with
-        | Some mp =>
-          if LabelMap.mem (elt:=unit) (Name f, Local 0) mp
-            then None
-            else Some (LabelMap.add (Name f, Local 0) tt mp)
-        | None => None
-      end) fs None = None.
+  (** Relate the above definitions to what [StructuredModule] wants. *)
+  Theorem makeVcs_correct : forall mn fs0 fs (Hmn : mn <> "malloc"), functionsWf fs = true
+    -> vcs (makeVcs fs)
+    -> vcs (StructuredModule.makeVcs
+              (("malloc", "malloc", Programming.Precondition mallocS None) :: nil) fs0
+      (map (fun p => match p with
+                       | {| FName := f; FVars := ns; FReserved := res;
+                         FPrecondition := pre; FBody := ch |} =>
+                       (f, pre, fun im' H => toCmd ch mn H ns res)
+                     end)
+      (map compileFunction fs))).
   Proof.
     induction fs; simpl; intuition.
+    apply andb_prop in H; intuition.
+    unfold functionWf in H2.
+    unfold compileFunction at 1.
+
+    repeat match goal with
+             | [ H : _ && _ = true |- _ ] => apply andb_true_iff in H; destruct H
+             | [ H : negb _ = true |- _ ] => apply negb_true_iff in H
+             | [ _ : context[if ?E then _ else _] |- _ ] => destruct E; try discriminate
+             | [ H : context[match ?E with None => _ | _ => _ end] |- _ ] => case_eq E; intros;
+               match goal with
+                 | [ H' : _ = _ |- _ ] => rewrite H' in *
+               end; try discriminate
+           end.
+    simpl.
+    wrap0.
+
+    post; clear_fancier.
+    assert (In "rp" ("rp" :: Formals a)) by (simpl; tauto).
+    assert (~In "rp" (Formals a))
+      by (intro; eapply In_notInList; try apply H1; eauto using in_or_app).
+    change (sel x1) with x1 in *.
+    unfold lvalIn, regInL in *; simpl in H1.
+    change (LvMem (Indir Sp (natToW O))) with (LvMem (Indir Sp (variablePosition ("rp" :: Formals a) "rp"))) in *.
+    evaluate auto_ext.
+
+    post.
+    assert (forall x4 x v, In x (map (fun s : string => (s ++ "0")%string) (Formals a ++ Locals a) ++ SpecVars a)
+      -> formals x2 (Formals a) x0 x
+      = formals (upd (merge x2 x4 ("rp" :: Formals a)) "rp" v)
+      (Formals a) x0 x).
+    intros.
+    apply in_app_or in H; intuition idtac.
+    apply in_map_iff in H29; destruct H29; intuition subst.
+
+    Lemma append0_invert : forall x y,
+      (x ++ "0" = y ++ "0")%string
+      -> x = y.
+    Proof.
+      induction x; destruct y; simpl in *; intuition.
+      destruct y; discriminate.
+      destruct x; discriminate.
+      injection H; clear H; intros; subst.
+      f_equal; auto.
+    Qed.
+
+    Lemma formals_switch : forall V V' x xs fE,
+      (In x xs -> sel V x = sel V' x)
+      -> formals V xs fE (x ++ "0")%string = formals V' xs fE (x ++ "0")%string.
+    Proof.
+      induction xs; simpl; intuition.
+      unfold fo_set.
+      destruct (string_dec (x ++ "0")%string (a ++ "0")%string); subst; auto.
+      apply append0_invert in e; subst.
+      f_equal; auto.
+    Qed.
+
+    apply formals_switch.
+    apply in_app_or in H30; intuition idtac.
+    rewrite sel_upd_ne.
+    symmetry; apply sel_merge.
+    simpl; tauto.
+    intro; subst.
+    eauto using in_or_app, In_notInList.
+    simpl in H29; intuition subst.
+    rewrite sel_upd_ne.
+    symmetry; apply sel_merge.
+    simpl; tauto.
+
+    Lemma NoDup_unapp : forall A (ls2 ls1 : list A),
+      NoDup (ls1 ++ ls2)
+      -> forall x, In x ls1 -> In x ls2 -> False.
+    Proof.
+      induction ls1; inversion 1; simpl; intuition (subst; eauto using in_or_app).
+    Qed.
+
+    exfalso; eauto using NoDup_unapp, NoDup_remove_1.
+
+    Lemma anyZero_duh : forall s, anyZero (s ++ "0")%string = true.
+    Proof.
+      induction s; simpl; intuition.
+      destruct a.
+      rewrite IHs.
+      repeat match goal with
+               | [ |- (if ?E then _ else _) = _ ] => destruct E; auto
+             end.
+    Qed.
+
+    Lemma formals_irrel : forall V V' x xs fE,
+      anyZero x = false
+      -> formals V xs fE x = formals V' xs fE x.
+    Proof.
+      induction xs; simpl; intuition.
+      unfold fo_set.
+      destruct (string_dec x (a ++ "0")%string); subst; auto.
+      rewrite anyZero_duh in H; discriminate.
+    Qed.
+
+    Lemma anyZeros_correct : forall x xs, anyZeros xs = false
+      -> In x xs
+      -> anyZero x = false.
+    Proof.
+      induction xs; simpl; intuition subst.
+
+      apply orb_false_iff in H; intuition.
+      apply orb_false_iff in H; intuition.
+    Qed.
+
+    eauto using formals_irrel, anyZeros_correct.
+
+    generalize dependent (map (fun s : string => (s ++ "0")%string) (Formals a ++ Locals a) ++ SpecVars a); intros.
+    clear_fancier.
+    change (locals ("rp" :: Formals a) x2 (S (S (S (S (S (S (S (S (length (Locals a))))))))))
+        (Regs x Sp))
+      with (locals_in ("rp" :: Formals a) x2 (S (S (S (S (S (S (S (S (length (Locals a))))))))))
+        (Regs x Sp)
+        ("_" :: Locals a) ("rp" :: Formals a ++ "_" :: Locals a) 7) in *.
+    assert (ok_in ("rp" :: Formals a) (S (S (S (S (S (S (S (S (length (Locals a))))))))))
+      ("_" :: Locals a) ("rp" :: Formals a ++ "_" :: Locals a) 7).
+    repeat split; unfold pr_var; auto; try omega.
+    simpl; omega.
+    simpl; constructor; auto.
+    intro.
+    apply in_app_or in H0; intuition subst.
+    eauto using In_notInList, in_or_app.
+    simpl in H26; intuition subst.
+    discriminate.
+    eapply In_notInList; try apply H1.
+    apply in_or_app; simpl; tauto.
+    apply NoDup_app.
+    eauto using NoDup_unapp1.
+    constructor; eauto using NoDup_unapp2.
+    intros.
+
+    Theorem good_vars_sound : forall xs, good_vars xs = true
+      -> List.Forall good_fo_var xs.    
+    Proof.
+      induction xs; simpl; intuition.
+      destruct a.
+      constructor; auto; constructor.
+      repeat match goal with
+               | [ _ : match ?E with _ => _ end = _ |- _ ] => destruct E; auto
+             end; constructor; auto; discriminate || constructor.
+    Qed.
+
+    intro.
+    apply good_vars_sound in H11.
+    eapply Forall_forall in H11; try eassumption.
+    destruct H11.
+    intros.
+    intro.
+    simpl in H26; intuition subst.
+    apply good_vars_sound in H12.
+    eapply Forall_forall in H12; try eassumption.
+    destruct H12.
+    eauto using NoDup_unapp.
+    simpl length; omega.
+    assert (In "rp" ("rp" :: Formals a ++ "_" :: Locals a)) by (simpl; tauto).
+    change (sel x2) with x2 in *.
+    unfold lvalIn, regInL in *; simpl in H25.
+    change (LvMem (Indir Sp (natToW O))) with (LvMem (Indir Sp (variablePosition ("rp" :: Formals a ++ "_" :: Locals a) "rp"))) in *.
+    clear H24.
+    evaluate auto_ext.
+    fold (@app pr_var) in *.
+    descend.
+    rewrite sel_eta.
+    step auto_ext.
+    etransitivity; [ apply himp_star_comm | ]; apply himp_star_frame; try reflexivity.
+    eapply weaken_predD; eauto.
+    eauto.
+    step auto_ext.
+    descend; step auto_ext.
+    instantiate (1 := x6).
+    change (locals ("rp" :: Formals a) x6
+        (S (S (S (S (S (S (S (S (Datatypes.length (Locals a)))))))))) (Regs x Sp))
+      with (locals_out ("rp" :: Formals a) x6
+        (S (S (S (S (S (S (S (S (Datatypes.length (Locals a))))))))))
+        (Regs x Sp) ("_" :: Locals a) ("rp" :: Formals a ++ "_" :: Locals a) 7).
+    assert (ok_out ("rp" :: Formals a)
+      (S (S (S (S (S (S (S (S (Datatypes.length (Locals a))))))))))
+      ("_" :: Locals a) ("rp" :: Formals a ++ "_" :: Locals a) 7).
+    repeat split; unfold pr_var; auto; try omega.
+    simpl; omega.
+    simpl length; omega.
+    rewrite sel_eta.
+    descend; step auto_ext.
+    eapply weaken_predD; eauto.
+    simpl; intuition (subst; eauto).
+    unfold fo_set.
+    destruct (string_dec x6 "result"); subst; auto.
+    symmetry; auto.
+
+
+    post.
+    generalize dependent (map (fun s : string => (s ++ "0")%string) (Formals a ++ Locals a) ++ SpecVars a); intros.
+    clear_fancier.
+    clear H24.
+    descend.
+    repeat rewrite sel_eta in *.
+    step auto_ext.
+    Focus 2.
+    apply himp_star_frame; try reflexivity.
+    eapply normalize_sound_fwd; eauto using notsInList_true.
+
+    Lemma formals_grab : forall V x xs fE,
+      In x xs
+      -> formals V xs fE (x ++ "0")%string = Dyn (sel V x).
+    Proof.
+      induction xs; simpl; intuition (subst; eauto).
+      unfold fo_set.
+      destruct (string_dec (x ++ "0")%string (x ++ "0")%string); subst; congruence.
+      unfold fo_set.
+      destruct (string_dec (x ++ "0")%string (a ++ "0")%string); subst; auto.
+      apply append0_invert in e; subst.
+      auto.
+    Qed.
+
+    Lemma vars_ok_formals : forall V xs fE,
+      vars_ok (formals V xs fE) V (vars0 xs).
+    Proof.
+      unfold vars_ok, vars0; induction xs; simpl; intuition.
+
+      destruct (string_dec a x); subst.
+      injection H; clear H; intros; subst; simpl.
+      unfold fo_set.
+      destruct (string_dec (x ++ "0") (x ++ "0")); tauto.
+      destruct (in_dec string_dec x xs); try discriminate.
+      injection H; clear H; intros; subst; simpl.
+      unfold fo_set.
+      destruct (string_dec (x ++ "0") (a ++ "0")).
+      apply append0_invert in e; congruence.
+      auto using formals_grab.
+    Qed.
+
+    apply vars_ok_formals.
+    step auto_ext.
+    step auto_ext.
+    descend; step auto_ext.
+    rewrite sel_eta.
+    descend; step auto_ext.
+    descend; step auto_ext.
+    eapply normalize_sound_bwd; eauto using notsInList_true.
+
+
+    hnf; auto.
+    intros.
+    apply in_app_or in H; intuition eauto using in_or_app.
+    apply in_or_app; right; simpl; tauto.
+
+    apply in_app_or in H0; intuition eauto using in_or_app, In_notInList.
+    simpl in H; intuition (subst; eauto using in_or_app, In_notInList).
+    discriminate.
+
+    rewrite Hndts in *; auto.
+
+    unfold vars0 in *.
+    destruct (in_dec string_dec x (Formals a)); auto; try congruence.
+    injection H; clear H; intros; subst; simpl.
+    apply H20.
+    apply in_or_app; left.
+    apply in_map_iff; eauto using in_or_app.
+
+    eauto using notsInList_true.
+
+    apply good_vars_sound in H14.
+    eapply Forall_forall in H14; eauto.
+
+    subst.
+    eapply notsInList_true in H15.
+    tauto.
+    eauto.
+    simpl; tauto.
+
+    apply in_app_or in H25; intuition idtac.
+    apply in_map_iff in H20; destruct H20; intuition subst.
+    apply in_app_or in H27; intuition idtac.
+    eapply notsInList_true in H15.
+    tauto.
+    apply H.
+    right.
+    apply in_or_app; left.
+    apply in_map_iff.
+    eauto using in_or_app.
+    eapply notsInList_true in H15.
+    tauto.
+    apply H.
+    right.
+    apply in_or_app; left.
+    apply in_map_iff.
+    eauto using in_or_app.
+    eapply notsInList_true in H15.
+    tauto.
+    apply H.
+    right.
+    apply in_or_app; auto.
+
+    apply good_vars_sound in H13.
+    eapply Forall_forall in H13; eauto.
+
+    apply in_app_or in H0; intuition idtac.
+    apply in_map_iff in H; destruct H; intuition subst.
+    assert (anyZero (x ++ "0")%string = true) by apply anyZero_duh.
+    rewrite H0 in H.
+    discriminate.
+
+    eauto using In_notInList.
+
+    eapply In_notInList; eauto.
+
+    eapply In_notInList; eauto.
+
+    apply in_app_or in H0; intuition eauto using In_notInList.
+    apply in_map_iff in H; destruct H; intuition subst.
+    assert (anyZero (x ++ "0")%string = true) by apply anyZero_duh.
+    rewrite H0 in H.
+    discriminate.
+
+    rewrite Hndts in *; assumption.
+
+    apply LabelMap.find_1.
+
+    Lemma MapsTo_fullImports' : forall m m' f sp (fs0 : list (StructuredModule.function m'))
+                                      (acc : LabelMap.t assert),
+      m <> m'
+      -> LabelMap.MapsTo (labl m f) sp acc
+      -> LabelMap.MapsTo (labl m f) sp (List.fold_left (fun m p => let '(f, pre, _) := p in
+         LabelMap.add (m', Global f) pre m) fs0 acc).
+    Proof.
+      induction fs0; simpl; intuition.
+      destruct a as [ [ ] ]; simpl in *.
+      eauto.
+    Qed.
+
+    Lemma MapsTo_fullImports : forall m m' f sp imps fs0,
+      m <> m'
+      -> LabelMap.MapsTo (labl m f) sp (importsMap imps)
+      -> LabelMap.MapsTo (labl m f) sp (fullImports (modName := m') imps fs0).
+    Proof.
+      intros; apply MapsTo_fullImports'; auto.
+    Qed.
+
+    apply MapsTo_fullImports; auto.
+    apply LabelMap.add_1; reflexivity.
+
+    apply in_or_app; simpl; tauto.
+
+    apply in_app_or in H0; intuition idtac.
+    apply good_vars_sound in H12.
+    eapply Forall_forall in H12; eauto.
+    destruct H12.
+    apply good_vars_sound in H11.
+    eapply Forall_forall in H11; eauto.
+    destruct H11.
+
+    unfold vars0.
+    destruct (in_dec string_dec "_" (Formals a)); auto.
+    apply good_vars_sound in H12.
+    eapply Forall_forall in H12; eauto.
+    destruct H12.    
   Qed.
 
-  Theorem NoDupFunc_out : forall fs (mp : LabelMap.t unit),
-    match (List.fold_left (fun mOpt f =>
-      match mOpt with
-        | None => None
-        | Some mp => let k := (Name f, Local 0) in
-          if LabelMap.mem k mp then None
+
+  (** * Modules *)
+
+  (** A named group of functions *)
+  Record module := {
+    MName : string;
+    Functions : list function
+  }.
+
+  (** Generating a full module *)
+  Section compileModule.
+    Variable m : module.
+
+    Definition compileModule : XCAP.module :=
+      bmodule_ (("malloc", "malloc", Programming.Precondition mallocS None) :: nil)
+               (MName m) (map compileFunction (Functions m)).
+
+    Lemma preserve_None : forall fs,
+      fold_left
+      (fun (mOpt : option (LabelMap.t unit)) (f : function) =>
+        match mOpt with
+          | Some mp =>
+            if LabelMap.mem (elt:=unit) (Name f, Local 0) mp
+              then None
+              else Some (LabelMap.add (Name f, Local 0) tt mp)
+          | None => None
+        end) fs None = None.
+    Proof.
+      induction fs; simpl; intuition.
+    Qed.
+
+    Theorem NoDupFunc_out : forall fs (mp : LabelMap.t unit),
+      match (List.fold_left (fun mOpt f =>
+        match mOpt with
+          | None => None
+          | Some mp => let k := (Name f, Local 0) in
+            if LabelMap.mem k mp then None
+              else Some (LabelMap.add k tt mp)
+        end) fs (Some mp)) with
+        | None => False
+        | Some _ => True
+      end
+      -> match (List.fold_left (fun mOpt (p : StructuredModule.function (MName m)) => let '(modl, _, _) := p in
+        match mOpt with
+          | None => None
+          | Some m => let k := (modl, Local 0) in
+            if LabelMap.mem k m then None
+              else Some (LabelMap.add k tt m)
+        end) (map (fun p => match p with
+                              | {| FName := f; FVars := ns; FReserved := res;
+                                FPrecondition := pre; FBody := ch |} =>
+                              (f, pre, fun im' H => toCmd ch (MName m) H ns res)
+                            end)
+        (map compileFunction fs)) (Some mp)) with
+           | None => False
+           | Some _ => True
+         end.
+    Proof.
+      induction fs as [ | [ ] ]; simpl; intuition.
+
+      unfold compileFunction; simpl.
+      destruct (boundVars Precondition0); simpl.
+      destruct (boundVars Postcondition0); simpl.
+      destruct (LabelMap.mem (Name0, Local 0) mp).
+      rewrite preserve_None in *; tauto.
+      apply IHfs; auto.
+      destruct (LabelMap.mem (Name0, Local 0) mp).
+      rewrite preserve_None in *; tauto.
+      apply IHfs; auto.
+      destruct (LabelMap.mem (Name0, Local 0) mp).
+      rewrite preserve_None in *; tauto.
+      apply IHfs; auto.
+    Qed.
+
+    Hypothesis NoDupFunc :
+      match (List.fold_left (fun mOpt f =>
+        match mOpt with
+          | None => None
+          | Some mp => let k := (Name f, Local 0) in
+            if LabelMap.mem k mp then None
             else Some (LabelMap.add k tt mp)
-      end) fs (Some mp)) with
-      | None => False
-      | Some _ => True
-    end
-    -> match (List.fold_left (fun mOpt (p : StructuredModule.function (MName m)) => let '(modl, _, _) := p in
-      match mOpt with
-        | None => None
-        | Some m => let k := (modl, Local 0) in
-          if LabelMap.mem k m then None
-            else Some (LabelMap.add k tt m)
-      end) (map (fun p => match p with
-                            | {| FName := f; FVars := ns; FReserved := res;
-                              FPrecondition := pre; FBody := ch |} =>
-                            (f, pre, fun im' H => toCmd ch (MName m) H ns res)
-                          end)
-      (map compileFunction fs)) (Some mp)) with
-         | None => False
-         | Some _ => True
-       end.
-  Proof.
-    induction fs as [ | [ ] ]; simpl; intuition.
+        end) (Functions m) (Some (LabelMap.empty unit))) with
+        | None => False
+        | Some _ => True
+      end.
 
-    unfold compileFunction; simpl.
-    destruct (boundVars Precondition0); simpl.
-    destruct (boundVars Postcondition0); simpl.
-    destruct (LabelMap.mem (Name0, Local 0) mp).
-    rewrite preserve_None in *; tauto.
-    apply IHfs; auto.
-    destruct (LabelMap.mem (Name0, Local 0) mp).
-    rewrite preserve_None in *; tauto.
-    apply IHfs; auto.
-    destruct (LabelMap.mem (Name0, Local 0) mp).
-    rewrite preserve_None in *; tauto.
-    apply IHfs; auto.
-  Qed.
+    Hypothesis FuncsWf : functionsWf (Functions m) = true.
+    Hypothesis FuncsVcs : vcs (makeVcs (Functions m)).
+    Hypothesis ModName : MName m <> "malloc".
 
-  Hypothesis NoDupFunc :
-    match (List.fold_left (fun mOpt f =>
-      match mOpt with
-        | None => None
-        | Some mp => let k := (Name f, Local 0) in
-          if LabelMap.mem k mp then None
-          else Some (LabelMap.add k tt mp)
-      end) (Functions m) (Some (LabelMap.empty unit))) with
-      | None => False
-      | Some _ => True
-    end.
+    (** Final correctness theorem *)
+    Theorem compileModule_ok : moduleOk compileModule.
+    Proof.
+      intros; apply bmoduleOk; auto.
 
-  Hypothesis FuncsWf : functionsWf (Functions m) = true.
-  Hypothesis FuncsVcs : vcs (makeVcs (Functions m)).
-  
-  (** Final correctness theorem *)
-  Theorem compileModule_ok : moduleOk compileModule.
-  Proof.
-    intros; apply bmoduleOk; auto.
+      Opaque string_dec.
+      simpl.
+      destruct (string_dec "malloc" (MName m)); congruence.
 
-    apply NoDupFunc_out; auto.
+      apply NoDupFunc_out; auto.
 
-    apply makeVcs_correct; auto.
-  Qed.
-End compileModule.
+      apply makeVcs_correct; auto.
+    Qed.
+  End compileModule.
+End dts.
